No more axiom in safety proof of poly1305

compiler/proof_vec/poly1305_avx_5xp_safe_proof.ec
@@ -1,40 +1,31 @@
 require import AllCore List Jasmin_model Int IntDiv CoreMap Poly1305_avx_5xp_safe.
 
-op is_align : wsize -> W64.t -> bool.
 
-op valid_range (w:wsize) (mem:global_mem_t) (ptr:W64.t) (len:int) =
-  forall i, i < len => is_valid mem (ptr + W64.of_int (wsize_i w * i)) w.
-
-axiom valid_range_size_le w1 w2 mem ptr len : 
-   wsize_i w1 <= wsize_i w2 => 
-   valid_range w2 mem ptr len =>
-   valid_range w1 mem ptr (len * wsize_i w2 %/ wsize_i w1).
-
-axiom valid_range_size_ge w1 w2 mem ptr len1 len2 :
-  is_align w2 ptr => 
-  wsize_i w1 <= wsize_i w2 =>  
-  (wsize_i w2 %/ wsize_i w1) * len2 <= len1 =>
-  valid_range w1 mem ptr len1 =>
-  valid_range w2 mem ptr len2.
-
-lemma ult_of_int x y :
-   (W64.of_int x \ult W64.of_int y) = (x %% W64.modulus < y %% W64.modulus).
-proof. by rewrite W64.ultE /= !of_uintK. qed.
-
-hint simplify ult_of_int.
 
 (*
-(* TODO : move this *)  
-lemma is_init_Some4 (t:'a Array4.t) : is_init (map Some t).
-proof. by cbv delta. qed.
+lemma valid_range_add32 mem ptr :
+  valid_range W64 mem ptr 8 =>
+  valid_range W64 mem ptr 4 /\
+  valid_range W64 mem (ptr + W64.of_int 32) 4.
+proof.
+  move=> hv;split.
+  + by apply: valid_range_le hv.
+  by apply (valid_range_add 4 W64 mem ptr 8).
+qed.
 
-lemma is_init_Some5 (t:'a Array5.t) : is_init (map Some t).
-proof. by cbv delta. qed.
-
-hint simplify (is_init_Some4, is_init_Some5)@0.
+lemma valid_range_add16 mem ptr :
+  valid_range W64 mem ptr 4 =>
+  valid_range W64 mem ptr 2 /\
+  valid_range W64 mem (ptr + W64.of_int 16) 2.
+proof.
+  move=> hv;split.
+  + by apply: valid_range_le hv.
+  by apply (valid_range_add 2 W64 mem ptr 4).
+qed.
 *)
 
 
+(* ----------------------------------------------------------------------------- *)
 hoare packS : M.pack : M.safe /\ valid_range W64 Glob.mem y 2 ==> M.safe.
 proof. 
   proc; wp; skip => /> &1 _ hv. 
@@ -64,21 +55,6 @@ proof. by proc; wp; skip. qed.
 hoare addS : M.add : M.safe ==> M.safe.
 proof. by proc; unroll for 2; wp; skip. qed.
 
-(* TODO: move this *)
-
-lemma nltgeE (x y: W64.t) : (! x \ult y) = (y \ule x).
-proof.
-  rewrite W64.ultE W64.uleE; smt ().
-qed.
-
-(* TODO: move this *)
-lemma to_uint_minus (x y: W64.t) : y \ule x => to_uint (x - y) = to_uint x - to_uint y.
-proof.
-  rewrite uleE=> hle.
-  rewrite to_uintD to_uintN modzDmr modz_small //.
-  apply bound_abs; have := W64.to_uint_cmp x; have := W64.to_uint_cmp y; smt ().
-qed.
-
 hoare load_lastS : M.load_last : 
    M.safe /\ valid_range W8 Glob.mem in_0 (W64.to_uint inlen) /\ is_align W64 in_0 ==> M.safe.
 proof. 
@@ -92,24 +68,24 @@ proof.
   + wp. 
     while (M.safe /\ is_init n /\ is_init m /\ is_init c /\ 
            valid_range W8 Glob.mem in_0 (to_uint inlen)).
-    + wp; skip; cbv delta => /> &1 _ _ _ _ _ hv.
-      move: (odflt _ _) => c1; rewrite W64.ultE => hlt.
-      by rewrite -(W64.to_uintK c1) hv.
+    + wp; skip => /> &1 _ _ _ _ _ hv.
+      move: (oget c{1}) => c1; rewrite W64.ultE => hlt.
+      by rewrite -(W64.to_uintK c1) (hv (to_uint c1)); smt (W64.to_uint_cmp).
     by wp; skip; cbv delta => />.
   wp. 
   while (M.safe /\ is_init n /\ is_init m /\ is_init c /\ 
          valid_range W8 Glob.mem in_0 (to_uint inlen)).
-  + wp; skip; cbv delta => /> &1 _ _ _ _ _ hv.
-    move: (odflt _ _) => c1; rewrite W64.ultE => hlt.
-    by rewrite -(W64.to_uintK c1) hv.
-  wp; skip; cbv delta => /> &1 _ hv ha _ _.
-  rewrite nltgeE => ^ hule; rewrite W64.uleE /= => hle.
+  + wp; skip => /> &1 _ _ _ _ _ hv.
+    move: (oget c{1}) => c1; rewrite W64.ultE => hlt.
+    by rewrite -(W64.to_uintK c1) (hv (to_uint c1)); smt (W64.to_uint_cmp).
+  wp; skip => /> &1 _ hv ha _ _.
+  rewrite -W64.uleNgt => ^ hule; rewrite W64.uleE /= => hle.
   split.
   + have h := (valid_range_size_ge W8 W64 Glob.mem{1} in_0{1} 
                    (to_uint inlen{1}) 1 ha _ _ hv) => //.
     by have /= := h 0 _.
-  move=> i; rewrite to_uint_minus 1:// (W64.to_uint_small 8) 1:// => h.
-  by apply hv => /#.
+  move=> i; rewrite to_uint_minus 1:// (W64.to_uint_small 8) 1:// => h /=.
+  apply (hv (8 + i))=> /#.
 qed. 
 
 hoare loadS: M.load : M.safe /\ valid_range W64 Glob.mem in_0 2 ==> M.safe.
@@ -158,44 +134,6 @@ proof.
   by call mulmod_u128S; wp; skip.
 qed.
 
-(* TODO: move this *)
-lemma valid_range_add (k:int) w mem ptr len :
-  k <= len =>   
-  valid_range w mem ptr len =>
-  valid_range w mem (ptr + W64.of_int (k * wsize_i w)) (len - k).
-proof.
-  move=> hk hv i hi /=. 
-  have -> : k * wsize_i w + wsize_i w * i = wsize_i w * (k + i) by ring.
-  apply hv => /#.
-qed.
-
-(* TODO: move this *)
-lemma valid_range_le (len1 len2:int) w mem ptr  :
-  len1 <= len2 =>   
-  valid_range w mem ptr len2 =>
-  valid_range w mem ptr len1.
-proof. by move=> hle hv i hlt; apply hv => /#. qed.
-  
-lemma valid_range_add32 mem ptr :
-  valid_range W64 mem ptr 8 =>
-  valid_range W64 mem ptr 4 /\
-  valid_range W64 mem (ptr + W64.of_int 32) 4.
-proof.
-  move=> hv;split.
-  + by apply: valid_range_le hv.
-  by apply (valid_range_add 4 W64 mem ptr 8).
-qed.
-
-lemma valid_range_add16 mem ptr :
-  valid_range W64 mem ptr 4 =>
-  valid_range W64 mem ptr 2 /\
-  valid_range W64 mem (ptr + W64.of_int 16) 2.
-proof.
-  move=> hv;split.
-  + by apply: valid_range_le hv.
-  by apply (valid_range_add 2 W64 mem ptr 4).
-qed.
-
 hoare first_blockS in0 : M.first_block : 
   M.safe /\ valid_range W64 Glob.mem in_0 8 /\ in_0 = in0 ==>
   M.safe /\ res.`2 = in0 + W64.of_int 64.
@@ -206,7 +144,8 @@ proof.
   call unpack_u128x2_to_u26x5x2S; wp.
   call mulmod_u128S; wp.
   call unpack_u128x2_to_u26x5x2S; wp.
-  skip => /> &1 _ /valid_range_add32 /> *; ring. 
+  skip => /> &1 _ h.  
+  by have := (valid_range_add_split 4 8 W64 Glob.mem{1} in_0{1} _ h).
 qed.
 
 hoare mulmod_add_u128_prefetchS : M.mulmod_add_u128_prefetch : 
@@ -233,30 +172,9 @@ proof.
   call add_u128S; wp.
   call mulmod_add_u128_prefetchS; wp.
   call mulmod_u128_prefetchS; wp.
-  skip => /> &1 _ /valid_range_add32 /> *; ring.
+  skip => /> &1 _ h.
+  by have := (valid_range_add_split 4 8 W64 Glob.mem{1} in_0{1} _ h).
 qed.
-
-(* TODO move this *)
-axiom is_align_add w ptr ofs: 
-  wsize_i w %| W64.to_uint ofs => is_align w ptr => is_align w (ptr + ofs).
-
-(*
-lemma to_uint0 : to_uint (W64.of_int 0) = 0.
-proof. by rewrite W64.to_uint_small. qed.
-
-lemma to_uint1 : to_uint (W64.of_int 1) = 1.
-proof. by rewrite W64.to_uint_small. qed.
-
-hint simplify (to_uint0, to_uint1)@0.
-
-axiom to_uint_bounded (w:W64.t) : 0 <= to_uint w < W64.modulus. 
-*)
-
-(* TODO : Move this *)
-
-lemma is_init_Some (a:'a) : is_init (Some a).
-proof. done. qed.
-hint simplify is_init_Some.
 
 hoare poly1305S : M.poly1305 :
     M.safe /\
@@ -275,7 +193,8 @@ proof.
     is_align W64 in_0 /\ 
     is_init s_out /\ is_init s_in /\ is_init s_inlen /\ is_init s_k /\ is_init r /\ 
     s_inlen = Some inlen /\ s_in = Some in_0).
-  + by wp; call clampS; wp; skip => /> &hr _ /valid_range_add16. 
+  + wp; call clampS; wp; skip => /> &hr _ h.
+    by have := valid_range_add_split 2 4 _ _ _ _ h. 
   seq 6 : (#pre /\ is_init s_r /\ is_init s_rx5).
   + by conseq />; unroll for 5; wp; skip; cbv delta.
   seq 9 : (#pre /\ is_init h /\ is_init b64 /\ 
@@ -340,7 +259,7 @@ proof.
     + rewrite to_uint_minus 1:W64.uleE /= 1:/# is_align_add //=.
       split; 1: smt().
       by have := valid_range_add 64 _ _ _ _ _ hv; smt (modz_ge0).
-    move=> ????. rewrite nltgeE W64.uleE /=.
+    move=> ????. rewrite -W64.uleNgt W64.uleE /=.
     smt (W64.to_uint_cmp).
       
   seq 16 : (M.safe /\
@@ -387,7 +306,7 @@ proof.
       have <- := modz_dvd (to_uint (oget s_inlen{hr})) 64 16 _; 1: done.
       by rewrite -divz_eq hv.
     have /= -> := W64.to_uint_and_mod 4 (oget s_inlen{hr}) _; 1: done.
-    move=> ? b16 ? ?; rewrite nltgeE W64.uleE /= => ? _ h1 _ _ _.
+    move=> ? b16 ? ?; rewrite -W64.uleNgt W64.uleE /= => ? _ h1 _ _ _.
     apply: valid_range_le h1; smt (W64.to_uint_cmp).
 
   call packS; wp. 
